src/Narcissus/Automation/AlignedAutomation.v
@@ -1,27 +1,10 @@
 Require Import Fiat.Narcissus.BinLib
         Fiat.Narcissus.Common.Specs
+        Fiat.Narcissus.Common.ComposeOpt
+        Fiat.Narcissus.Formats
         Fiat.Narcissus.Automation.Solver.
 
-Ltac start_synthesizing_encoder :=
-  lazymatch goal with
-  | |- CorrectAlignedEncoderFor ?Invariant ?Spec =>
-    try unfold Spec; try unfold Invariant
-  end;
-  (* Memoize any string constants *)
-  (*pose_string_hyps; *)
-  eexists; simpl; intros.
-
-Ltac align_encoder_step :=
-  first [
-      apply @CorrectAlignedEncoderForThenC
-    | apply @CorrectAlignedEncoderForDoneC
-    | apply CorrectAlignedEncoderForFormatList
-    | apply CorrectAlignedEncoderForFormatChar; eauto
-    | apply CorrectAlignedEncoderForFormat2Char; eauto
-    | apply CorrectAlignedEncoderForFormatNat].
-
-Ltac align_encoder :=
-  repeat align_encoder_step.
+Require Import Bedrock.Word.
 
 Ltac start_synthesizing_decoder :=
   match goal with
@@ -42,6 +25,7 @@ Ltac align_decoders_step :=
     | eapply @Return_DecodeMEquivAlignedDecodeM].
 
 Ltac align_decoders := repeat align_decoders_step.
+
 Locate Ltac normalize_compose .
 Ltac synthesize_aligned_decoder :=
   start_synthesizing_decoder;
@@ -54,6 +38,167 @@ Ltac synthesize_aligned_decoder :=
   | ];
   cbv beta; align_decoders.
 
+Lemma length_encode_word' sz :
+  forall (w : word sz) (b : ByteString),
+    bin_measure (encode_word' _ w b) = sz + bin_measure b.
+Proof.
+  simpl; intros.
+  rewrite <- (ByteStringToBoundedByteString_BoundedByteStringToByteString_eq b).
+  rewrite !length_ByteString_ByteStringToBoundedByteString_eq.
+  rewrite <- length_encode_word' with (w := w).
+  induction sz; intros;
+    rewrite (shatter_word w); simpl.
+  - reflexivity.
+  - rewrite Core.length_ByteString_enqueue, <- IHsz.
+    rewrite (ByteStringToBoundedByteString_BoundedByteStringToByteString_eq b).
+    rewrite <- (ByteStringToBoundedByteString_BoundedByteStringToByteString_eq (encode_word' _ _ _)).
+    rewrite ByteString_enqueue_ByteStringToBoundedByteString_eq.
+    rewrite !length_ByteString_ByteStringToBoundedByteString_eq.
+    rewrite Core.length_ByteString_enqueue; reflexivity.
+Qed.
+
+Lemma length_ByteString_word
+  : forall (sz : nat) (w : word sz) (b : ByteString) (ctx ctx' : CacheFormat),
+    format_word w ctx ↝ (b, ctx') -> length_ByteString b = sz.
+Proof.
+  unfold WordOpt.format_word; simpl.
+  intros; computes_to_inv; injections.
+  rewrite length_encode_word'; simpl.
+  unfold ByteString_id, length_ByteString; simpl; omega.
+Qed.
+
+Lemma length_ByteString_unused_word
+  : forall (sz : nat) (b : ByteString) (ctx ctx' : CacheFormat),
+    format_unused_word sz ctx ↝ (b, ctx') -> length_ByteString b = sz.
+Proof.
+  unfold format_unused_word, format_unused_word';
+    intros; computes_to_inv; injections.
+  rewrite length_encode_word'; simpl.
+  unfold ByteString_id, length_ByteString; simpl; omega.
+Qed.
+
+Lemma length_ByteString_bool
+  : forall (b : bool) (bs : ByteString) (ctx ctx' : CacheFormat),
+    format_bool b ctx ↝ (bs, ctx') -> length_ByteString bs = 1.
+Proof.
+  unfold format_bool, format_unused_word';
+    intros; computes_to_inv; injections.
+  reflexivity.
+Qed.
+
+Locate "ThenC".
+
+Lemma length_ByteString_compose:
+  forall (format1 format2 : CacheFormat -> Comp (ByteString * CacheFormat))
+         (b : ByteString) (ctx ctx' : CacheFormat)
+         (n n' : nat),
+    (forall (ctx0 : CacheFormat) (b0 : ByteString) (ctx'0 : CacheFormat),
+        format1 ctx0 ↝ (b0, ctx'0) -> length_ByteString b0 = n) ->
+    (forall (ctx0 : CacheFormat) (b0 : ByteString) (ctx'0 : CacheFormat),
+        format2 ctx0 ↝ (b0, ctx'0) -> length_ByteString b0 = n') ->
+    (format1 ThenC format2) ctx ↝ (b, ctx') ->
+    length_ByteString b = n + n'.
+Proof.
+  intros.
+  unfold compose, Bind2 in H1; computes_to_inv.
+  destruct v; destruct v0; simpl in *; injections.
+  erewrite length_ByteString_enqueue_ByteString, H, H0; eauto with arith.
+Qed.
+
+Ltac eapply_in_hyp lem :=
+  match goal with
+  | H:_ |- _ => eapply lem in H; [ | clear H | .. | clear H]
+  end.
+
+Ltac associate_for_ByteAlignment :=
+  eapply @Guarded_CorrectAlignedEncoderThenCAssoc;
+  [clear; intros ce bs ce' Comp;
+   repeat first [ apply_in_hyp length_ByteString_word
+                | apply_in_hyp length_ByteString_unused_word
+                | apply_in_hyp length_ByteString_bool
+                | eapply_in_hyp length_ByteString_compose;
+                  [ | clear; intros | .. | clear; intros ]
+                | eassumption]; omega
+  | ].
+
+
+Lemma CollapseCorrectAlignedEncoderFormatWord
+      (addE_addE_plus :
+         forall ce n m, addE (addE ce n) m = addE ce (n + m))
+  : forall sz {sz'} (w' : word sz') k encoder,
+    CorrectAlignedEncoder
+      ((format_word (combine w' (wzero sz)))
+         ThenC k)
+      encoder
+    -> CorrectAlignedEncoder
+         ((format_unused_word sz)
+            ThenC (format_word w')
+            ThenC k)
+         encoder.
+Proof.
+  intros; eapply refine_CorrectAlignedEncoder; eauto.
+  intros; rewrite <- CollapseFormatWord; eauto.
+  unfold compose, Bind2; f_equiv.
+  unfold format_unused_word, format_unused_word'.
+  repeat computes_to_econstructor; eauto.
+Qed.
+
+Lemma refine_format_unused_word
+  : forall sz ce,
+    refine (format_unused_word sz ce) (format_word (wzero sz) ce).
+Proof.
+  intros; unfold format_unused_word, format_unused_word'.
+  repeat computes_to_econstructor; eauto.
+Qed.
+
+Lemma refine_format_bool
+  : forall b ce,
+    refine (format_bool b ce) (format_word (WS b WO) ce).
+Proof.
+  intros; unfold format_bool.
+  reflexivity.
+Qed.
+
+Ltac collapse_unaligned_words :=
+  intros; eapply refine_CorrectAlignedEncoder;
+  [ eauto ; intros; try set_refine_evar; repeat eapply refine_CollapseFormatWord; intros;
+    unfold format_nat; eauto using refine_format_bool, refine_format_unused_word;
+    reflexivity
+  | ].
+
+Ltac decompose_aligned_encoder :=
+  repeat first [
+           eapply @CorrectAlignedEncoderForIPChecksumThenC
+         | associate_for_ByteAlignment
+         | match goal with
+             |- context[ByteString_id] => apply @CorrectAlignedEncoderForThenC
+           end
+         | apply @CorrectAlignedEncoderForDoneC].
+
+Ltac start_synthesizing_encoder :=
+  lazymatch goal with
+  | |- CorrectAlignedEncoderFor ?Invariant ?Spec =>
+    try unfold Spec; try unfold Invariant
+  end;
+  (* Memoize any string constants *)
+  (*pose_string_hyps; *)
+  eexists; simpl; intros.
+
+Ltac align_encoder_step :=
+  first
+    [ apply CorrectAlignedEncoderForFormatList
+    | apply CorrectAlignedEncoderForFormatChar; eauto
+    | apply CorrectAlignedEncoderForFormatNat
+    | intros; eapply CorrectAlignedEncoderForFormatNChar with (sz := 2); eauto
+    | intros; eapply CorrectAlignedEncoderForFormatNChar with (sz := 3); eauto
+    | intros; eapply CorrectAlignedEncoderForFormatNChar with (sz := 4); eauto
+    | intros; eapply CorrectAlignedEncoderForFormatNChar with (sz := 5); eauto
+    | collapse_unaligned_words].
+
+Ltac align_encoder :=
+  repeat align_encoder_step.
+
 Ltac synthesize_aligned_encoder :=
   start_synthesizing_encoder;
-  align_encoder.
+  decompose_aligned_encoder;
+  repeat align_encoder_step.
